#import "/module/module.typ": *
#show: module

#tag("analytic-struct-product") ç§¯ç©ºé—´
#indent[
  ä¸å¯¹ç§°æ€§: $V != W$ ==> æ²¡æœ‰ $V âŠ™ W$

  åªå¥½ä½¿ç”¨ $(âŠ™^n V) âŠ— (âŠ™^m W)$ å’Œåå¾®åˆ†

  something like

  $ #d^l f (x,y) : v,w â‡ sum_(n + m = l) binom(l,n,m) (âˆ‚^(n+m) f)/(âˆ‚ v^n âˆ‚ w^m) (x,y) (v^n âŠ— w^m) $
]
#tag("mulitplication-analytic")
#indent[
  - $ğ•‚ -> ğ•‚$
  #indent[
    $ (sum_(n âˆˆ â„•) a_n v^n) (sum_(m âˆˆ â„•) b_m v^m) = sum_(l âˆˆ â„•) c_l v^l $

    with $c_l = sum_(n+m=l) a_n b_m$

    æ”¶æ•›åŠå¾„è‡³å°‘æ˜¯ $min(R_A,R_B)$

    (è”ç³»äº Cauchy product. å°è¯•å¯»æ‰¾æ›´å¥½çš„è¯æ˜æ–¹æ³•)

    $c_1 = a_1 b_0 + a_0 b_1$

    æ¢å¤å¾®åˆ†ä¸­çš„ $1/n!$, $sum a_n v^n âˆ¼ sum 1/(n!) #d^n f (x) (v^n)$

    ==> #tag("Leibniz-law-1d")
    
    $#d (f g)(x) (v) = (#d f(x) (v)) g(x) + f(x) (#d g(x) (v))$, or 

    $(âˆ‚ (f g))/(âˆ‚ v) = (âˆ‚ f)/(âˆ‚ v) g + f (âˆ‚ g)/(âˆ‚ v) $, or
    
    $(f g)' = f' g + f g'$
  ]
  - $ğ•‚^d -> ğ•‚$
  #indent[
    $ (sum_(n âˆˆ â„•) a_n v^n) (sum_(m âˆˆ â„•) b_m v^m) = sum_(l âˆˆ â„•) c_l v^l $
    
    æ”¶é›† $n+m$ é‡å¼ é‡ $A_n (v_1 â‹¯ v_n) B_m (v_(n+1) â‹¯ v_(n+m))$
    
    let $forall i, v_i = v$ å¾—åˆ° $n+m$ å¤šé¡¹å¼ $A_n (v^n) B_m (v^m)$

    ==> $C_l (v^l) = sum_(n+m=l) A_n (v^n) B_m (v^m)$

    $C_1 v = A_1 (v) B_0 + A_0 B_1 (v)$

    ==> #tag("Leibniz-law") $(âˆ‚ (f g))/(âˆ‚ v) = (âˆ‚ f)/(âˆ‚ v) g + f (âˆ‚ g)/(âˆ‚ v) $
  ]
]
#tag("mulitplication-inverse-analytic")
#indent[
  let $f : ğ•‚^d -> ğ•‚$, $f = sum A_n (v^n)$, $A_0 != 0$

  use $f = 1 - g$ and $1/(1 - g) = 1 + g + g^2 + â‹¯$

  or ç›´æ¥è®¡ç®—

    let $1/f = sum B_m v^m$, $1/f â‹… f = 1$, use ä¹˜æ³•

    $m = 0$: $1 = A_0 B_0$

    $m >= 1$: $0 = C_l = sum_(n+m=l) A_n B_m$

    ==> $B_m = - 1/(A_0) sum_(n=1)^m A_n B_(m-n)$, use induction $B_0 ,â€¦, B_(m-1)$

  #tag("differential-of-multiplication-inverse") use Leibniz law 
  #indent[
    $0 = âˆ‚_(v) (1/f â‹… f) = âˆ‚_(v) (1/f) f + 1/f âˆ‚_(v) f ==> âˆ‚_(v) (1/f) = - 1/(f^2) âˆ‚_(v) f $, or

    $(1/f)' = - (f')/(f^2)$

    in particular, $(1/x)' = - 1/(x^2)$
  ]
  æ”¶æ•›åŠå¾„
  #indent[
    try å½’çº³è¯æ˜ $|B_m| <= R^m$

    $|A_0| |B_m| 
    &<= sum_(n=1)^m |A_n| |B_(m-n)| \ 
    &<= sum_(n=1)^m |A_n| R^(m-n) quad ("by induction" B_1 ,â€¦, B_(m-1)) \
    &= R^m sum_(n=1)^m |A_n| (1/R)^n \
    &<= R^m sum_(n=1)^âˆ |A_n| (1/R)^n$

    ä¸ºå®Œæˆå½’çº³, use $R$ with $1/(|A_0|) sum_(n=1)^âˆ |A_n| (1/R)^n <= 1$
  ]
]
#tag("compose-op-analytic")
#indent[
  - $ğ•‚ -> ğ•‚$
  #indent[
    let $f(y+w) = sum a_n v^n$, $g(x+v) = sum b_m w^m$
    
    with $a_0 = f(y) = f(g(x)) = f(b_0)$

    $f(g(x+v)) âˆ˜ 
    &= f(b_0 + sum_(m=1)^âˆ b_m v^m) \
    &= a_0 + sum_(n=1)^âˆ a_n (sum_(m=1)^âˆ b_m v^m)^n \
    &= c_0 + sum_(l=1)^âˆ c_l v^l$

    where å¤åˆåçš„ $v^l$ çš„æ‰€æœ‰å¯èƒ½æ¥æº 
    
    $v^l = (v^1)^(i_1) â‹¯ (v^l)^(i_l) = v^(1 â‹… i_1 + â‹¯ + l â‹… i_l)$ with $l = 1 â‹… i_1 + â‹¯ + l â‹… i_l$

    ä»è€Œåªèƒ½æ¥è‡ª for $k = 1 ,â€¦, l$ 
    
    $(b_1 v + â‹¯ + b_l v^l)^k 
    = sum_(i_1 + â‹¯ + i_l = k) binom(k,i_1,...,i_l) b_1^(i_1) â‹¯ b_l^(i_l)$ (cf. #link(<multi-combination>)[])

    ==> 
    $ 
      c_l v^l = 
      sum_(k = 1 ,â€¦, l) 
      sum_(i_1 ,â€¦, i_l in â„• \ i_1 + â‹¯ + i_l = k \ 1 â‹… i_1 + â‹¯ + l â‹… i_l = l)
      binom(k, i_1 ,â€¦, i_l) a_k b_1^(i_1) â‹¯ b_l^(i_l) v^(1 â‹… i_1 + â‹¯ + l â‹… i_l) 
    $
    $c_1 = a_1 b_1$. å†™ä¸ºå¾®åˆ† #tag("chain-rule-1d") 
    
    $#d (f âˆ˜ g)(x) (v) = #d f (g(x)) (#d g(x) (v)) $, or 
    
    $(f âˆ˜ g)'(x) = f'(g(x)) g'(x)$
  ]
  - $ğ•‚^d -> ğ•‚^(d')$
  #indent[
    $ 
      C_l (v^l) = 
      sum_(k = 1 ,â€¦, l) 
      sum_(i_1 ,â€¦, i_l in â„• \ i_1 + â‹¯ + i_l = k \ 1 â‹… i_1 + â‹¯ + l â‹… i_l = l)
      binom(k,i_1,...,i_l) A_k (B_1^(i_1) â‹¯ B_l^(i_l) (v^(1 â‹… i_1 + â‹¯ + l â‹… i_l))) 
    $
    where $B_1^(i_1) â‹¯ B_l^(i_l) (v^(1 â‹… i_1 + â‹¯ + l â‹… i_l)) 
    = (B_1 (v^(âŠ™ 1)))^(âŠ™ i_1) âŠ™ â‹¯ âŠ™ (B_l (v^(âŠ™ l)))^(âŠ™ i_l)$

    $C_1 (v) = A_1 (B_1 (v))$, å†™ä¸ºå¾®åˆ†å°±æ˜¯ #tag("chain-rule")

    $#d (f âˆ˜ g)(x) (v) = #d f (g(x)) (#d g (x) (v)) $ 

    ä¸€èˆ¬çš„å†™ä¸ºå¾®åˆ†çš„å½¢å¼
    #indent[
      - $C_l âˆ¼ 1/(l!) #d^l (f âˆ˜ g)$ 
      
      - $A_k âˆ¼ 1/(k!) #d^k f$

      - $B_j âˆ¼ 1/(j!) #d^j g $
      
      in $#d^l (f âˆ˜ g) (x) (v^l) = "formula of" #d^k f , #d^j g$ 
      
      å°† $l! , 1/(k!) , (1/(j!))^(i_j)$ æå–
      
      ç½®äº $binom(k,i_1,...,i_l) = (k!)/(i_1! â‹¯ i_l!)$ 
      
      å¾—åˆ° $(l!)/((1!)^(i_1) â‹… i_1! â‹¯ (l!)^(i_l) â‹… i_l!)$ 
      (this is _not_ $(l!)/((1 â‹… i_1)! â‹¯ (l â‹… i_l)!) = binom(l , 1 â‹… i_1 ,â€¦, l â‹… i_l)$)
      $
        #d^l (f âˆ˜ g) = 
        sum_(k = 1 ,â€¦, l) 
        sum_(i_1 ,â€¦, i_l in â„• \ i_1 + â‹¯ + i_l = k \ 1 â‹… i_1 + â‹¯ + l â‹… i_l = l)
        (l!)/((1!)^(i_1) â‹… i_1! â‹¯ (l!)^(i_l) â‹… i_l!) 
        #d^k f (#d^1 g) ^(i_1) â‹¯ (#d^l g)^(i_l)
      $
    ]
  ]
]
#tag("inverse-analytic")
#indent[
  let $f âˆ¼ sum A_n (v^n)$, $ğ•‚^d -> ğ•‚^d$, $A_1 in GL(d,ğ•‚)$ 

  let $f^(-1) (y + v) = sum B_m (v^m)$

  - ä¸€é˜¶å¾®åˆ†è®¡ç®—. $f âˆ˜ f^(-1) = f^(-1) âˆ˜ f = ğŸ™ : v â‡ v$, use å¤åˆ
  #indent[
    $ğŸ™ (v) = sum C_l (v^l)$

    $C_0 = 0 \ C_1 = ğŸ™ \ C_l = 0 , forall l >= 2 $

    $ğŸ™ (v) = C_1 (v) = A_1 (B_1 (v)) ==> B_1 = A_1^(-1)$ by $A_1 in GL(d,ğ•‚)$
  ]
  - é«˜é˜¶å¾®åˆ†è®¡ç®—. use å½’çº³ for $B_1 ,â€¦, B_(l-1)$
  #indent[
    $B_l$ åªæ¥è‡ª 

    $i_1 = â‹¯ = i_(l-1) = 0$ and $i_l = 1$ ==> $1 â‹… i_1 + â‹¯ + l â‹… i_l = l$

    $i_1 + â‹¯ + i_l = 1$

    $binom(l,0,â€¦,l) = 1$

    ==> (çœç•¥ $(v^l)$)
    $
      0 
      &= C_l \
      &= A_1 B_l \
      &quad + sum_(k = 2 ,â€¦, l) 
      sum_(i_1 ,â€¦, i_l in â„• \ i_1 + â‹¯ + i_l = k \ 1 â‹… i_1 + â‹¯ + l â‹… i_l = l)
      binom(k,i_1,...,i_l) A_k B_1^(i_1) â‹¯ B_(l-1)^(i_(l-1))
    $
    $A_1 in GL$ 
    ==> 
    $
      B_l = - A_1^(-1) 
      sum_(k = 2 ,â€¦, l) 
      sum_(i_1 ,â€¦, i_l in â„• \ i_1 + â‹¯ + i_l = k \ 1 â‹… i_1 + â‹¯ + l â‹… i_l = l)
      binom(k,i_1,...,i_l) A_k B_1^(i_1) â‹¯ B_(l-1)^(i_(l-1)) 
    $
  ]
  ç”±äºå¯èƒ½ä¸æ”¶æ•›, $f âˆ¼ sum_(n >= 1) A_n (v^n)$ æ— æ³•ç›´æ¥ä½œä¸º $ğ•‚^d -> ğ•‚^d$ å‡½æ•°

  ä½†æ˜¯å¯ä»¥æ‰©å……åˆ° $f : â¨_(n = 1)^âˆ Lin(âŠ™^n ğ•‚^d -> ğ•‚^(d')) -> "self"$

  ä½¿å¾— $f âˆ˜ f^(-1) = f^(-1) âˆ˜ f = ğŸ™ "of" â¨_(n = 1)^âˆ Lin(âŠ™^n ğ•‚^d -> ğ•‚^(d'))$

  - é€†å‡½æ•°çš„æ”¶æ•›åŠå¾„éé›¶ (p.77 of @ref-4)
  #indent[
    *Reference* 
    $
      B_l = - A_1^(-1) 
      sum_(k = 2 ,â€¦, l) 
      sum_(i_1 ,â€¦, i_l in â„• \ i_1 + â‹¯ + i_l = k \ 1 â‹… i_1 + â‹¯ + l â‹… i_l = l)
      binom(k,i_1,...,i_l) A_k B_1^(i_1) â‹¯ B_(l-1)^(i_(l-1)) 
    $
    ==>
    $
      &|B_l| 
      &<= 1/(|A_1|) 
      sum_(k = 2 ,â€¦, l) 
      sum_(i_1 ,â€¦, i_l in â„• \ i_1 + â‹¯ + i_l = k \ 1 â‹… i_1 + â‹¯ + l â‹… i_l = l)
      binom(k,i_1,...,i_l) |A_k| |B_1|^(i_1) â‹¯ |B_(l-1)|^(i_(l-1))  
    $
    use $binom(k,i_1,...,i_l) âˆˆ â„_(>= 0)$ (indeed $âˆˆ â„•$)

    æ„é€  (å‡ ä¹) $â„_(>= 0)$ çš„éé›¶æ”¶æ•›åŠå¾„çš„å¹‚çº§æ•°æ§åˆ¶ $|A_k| <= a_k, |B_k| <= b_k$

    if by induction, for $A_2 ,â€¦, A_l$, $B_1 ,â€¦, B_(l-1)$, $|A_k| <= a_k$, $|B_j| <= b_j$
    #indent[  
      where $sum_(k >= 1) a_k v^k$ with $k >= 2 ==> a_k in â„_(>= 0)$ 
      
      å…¶é€†æ˜¯ $sum_(j >= 1) b_j v^j$ with $j >= 1 ==> b_j in â„_(>= 0)$. $â„_(>= 0)$ to prove. æ”¶æ•›åŠå¾„éé›¶ to prove
      
      use case of $ğ•‚ -> ğ•‚$ 
      $ 
        b_l = - 1/(a_1) 
        sum_(k = 2 ,â€¦, l) 
        sum_(i_1 ,â€¦, i_l in â„• \ i_1 + â‹¯ + i_l = k \ 1 â‹… i_1 + â‹¯ + l â‹… i_l = l)
        binom(k,i_1,...,i_l) a_k b_1^(i_1) â‹¯ b_(l-1)^(i_(l-1)) 
      $
      to get $b_j >= 0$, use $a_1 < 0$
    ]
    ==> 
    $
      |B_l| 
      &<= 1/(|A_1|) 
      sum_(k = 2 ,â€¦, l) 
      sum_(i_1 ,â€¦, i_l in â„• \ i_1 + â‹¯ + i_l = k \ 1 â‹… i_1 + â‹¯ + l â‹… i_l = l)
      binom(k,i_1,...,i_l) |A_k| |B_1|^(i_1) â‹¯ |B_(l-1)|^(i_(l-1)) \
      &<= (-a_1)/(|A_1|) b_l
    $
    
    $|B_1| = 1/(|A_1|)$, $b_1 = 1/(-a_1)$

    to get $|B_l| <= b_l$, $|B_1| <= b_1$, use $a_1 = - |A_1| =: Î±$

    to get $k >= 2 ==> |A_k| <= a_k$, use $a_k = (sup_(k >= 2) {|A_k|^(1/k)})^k =: Î²^k$

    now prove å¹‚çº§æ•° $a_k$ çš„é€†å¹‚çº§æ•° $b_k$ æ”¶æ•›åŠå¾„éé›¶
    $
      sum_(n >= 1) a_k v^k 
      &= Î± v + sum_(n >= 2) Î²^k v^k \
      &âˆ¼ Î± v + 1/(1 - Î² v) - 1 - Î² v \
      &= Î± v + ((Î² v)^2)/(1- Î² v) 
    $
    let $f(v) = Î± v + ((Î² v)^2)/(1- Î² v) âˆ¼ sum a_k v^k$, $f^(-1)(v) = g(v) âˆ¼ sum b_j v^j$

    ä¸ºäº†æ±‚ $f$ çš„é€†æ˜ å°„ $f^(-1) = g$, è§£æ–¹ç¨‹ $Î± g(v) + ((Î² g(v))^2)/(1 - Î² g(v)) = v$ 
    
    ==> $g(v)$ çš„äºŒæ¬¡æ–¹ç¨‹, æœ‰ä¸¤ä¸ªæ ¹
    
    use $f(0) = 0 ==> g(0) = 0$, é€‰å–æ­£ç¡®çš„æ ¹
    
    $ g(v) = (-(Î± + Î² v) - ((Î± + Î² v)^2 + 4 Î² (Î² - Î±) v)^(1/2))/(2 Î² (Î² - Î±)) $
    
    use $(1+w)^(1/2) âˆ¼ sum_(n âˆˆ â„•) binom(1/2,n) w^n$ æ”¶æ•›åŠå¾„ $1$ ==> $g(v) âˆ¼ sum b_j v^j$ éé›¶æ”¶æ•›åŠå¾„ 
    
    use $|B_l| <= b_l$ ==> $sum B_j v^j$ éé›¶æ”¶æ•›åŠå¾„ 
      
    è™½ç„¶è¿™é‡Œæ— æ³•ç»™å‡ºç¡®åˆ‡çš„æ”¶æ•›åŠå¾„, ä½†æ˜¯å¯¹äºçº¯å¾®åˆ†æ–¹æ³•, å‹ç¼©ä¸åŠ¨ç‚¹åŸç†è¯æ˜é€†å‡½æ•°çš„æ–¹æ³•ä¹Ÿä¸èƒ½ç»™å‡ºç¡®åˆ‡çš„æå¤§å±€éƒ¨å¯é€†åŒºåŸŸ
  ]
]
#tag("differential-of-inverse") 

$ğŸ™ "of" "power series space" = f âˆ˜ f^(-1) \
==> ğŸ™ "of" GL = #d f (f^(-1)(x)) #d f^(-1)(x) \
==> #d f^(-1) (x) = (#d f (f^(-1)(x)))^(-1)$

or $(f^(-1))'(x) = 1/(f'(f^(-1)(x)))$

#tag("implicit-function")

use #link(<analytic-struct-product>)[]

$F(x,y) = 0$ and $(âˆ‚ F)/(âˆ‚ y)(x,y) in GL$

==> $F(x,f(x)) = 0$, $#d f (x) = - ((âˆ‚ F)/(âˆ‚ y))^(-1) (âˆ‚ F)/(âˆ‚ x) (x,f(x))$

å¾®åˆ†å’Œå¾®åˆ†å‡½æ•°çš„è®¡ç®—ä¸éœ€è¦é¢„å…ˆæœ‰çº§æ•°

- æœ‰é™ç‚¹å¤„æ”¶æ•›åŠå¾„ä¸ºé›¶çš„ $C^âˆ$ å‡½æ•°

  $ exp 1/(1-x^2)$ æ¥ä¸Š $0$ 

- å¤„å¤„ $C^âˆ$ ä½†å¤„å¤„æ”¶æ•›åŠå¾„ $0$ çš„å‡½æ•° 
#indent[
  #link("https://en.wikipedia.org/wiki/Non-analytic_smooth_function")[wiki: Non-analytic_smooth_function] 

  $ F(x) := sum_(k in â„•) e^(-sqrt(2^k)) cos(2^k x) $ 

  Since the series $sum_(k in â„•) e^(-sqrt(2^k)) (2^k)^n$ converges for forall $n in â„•$, this function is easily seen to be of class $C^âˆ$, by a standard inductive application of the Weierstrass M-test to demonstrate uniform convergence of each series of derivatives.

  We now show that $F(x)$ is not analytic at any dyadic rational multiple of $Ï€$, that is, at any $x := Ï€ â‹… p â‹… 2^(âˆ’q)$ with $p âˆˆ â„¤$ and $q âˆˆ â„•$. 

  Since the sum of the first q terms is analytic, we need only consider $F_(> q)(x) $, the sum of the terms with $k > q$. 

  For forall orders of derivation $n = 2^m$ with $m âˆˆ N $, $m â‰¥ 2$ and $m > q/2$ we have 

  $
    F^((n))_(>q) 
    &:= sum_(k âˆˆ â„• \ k > q) e^(-sqrt(2^k)) (2^k)^n cos(2^k x) \
    &= sum_(k âˆˆ â„• \ k > q) e^(-sqrt(2^k)) (2^k)^n \
    &>= e^(-n) n^(2 n) ("as" n -> âˆ )
  $

  where we used the fact that $cos(2^k x) = 1$ for forall $2^k > 2^q$, and we bounded the first sum from below by the term with $2^k = 2^(2 m) = n^2$. 

  As a consequence, at any such $x âˆˆ â„$, 

  $ limsup_(n -> âˆ) ((|F^((n))_(> q)|)/(n!))^(1/n) = âˆ $

  Since the set of analyticity of a function is an open set, and since dyadic rationals are dense, we conclude that $F_(> q)$, and hence $F$, is nowhere analytic in $â„$
]
- è¿ç»­ä½†å¤„å¤„ä¸å¯å¾® 
#indent[
  #link("https://en.wikipedia.org/wiki/Weierstrass_function")[wiki: Weierstrass_function] 

  $ f(x) = sum_(n =0)^âˆ a^n cos(b^n Ï€ x) $ 

  where $0 < a < 1$, $b$ is positive odd integer, and $a b > 1+ 3/2 Ï€$ 
]
- $k$ é˜¶å¯å¾®ä½†ä¸ $k+1$ é˜¶å¯å¾®: ä½¿ç”¨ Weierstrass å‡½æ•°çš„å„é˜¶ç§¯åˆ†

- $k$ é˜¶å¯å¾®ä½† $k$ é˜¶ä¸è¿ç»­å¯å¾® (è™½ç„¶ $k$ é˜¶å¯å¾®è•´å« $k-1$ é˜¶è¿ç»­å¯å¾®): ä½¿ç”¨ $x^2 sin 1/x$, $1$ é˜¶å¯å¾®ä½†ä¸ $1$ é˜¶è¿ç»­å¯å¾®, ä½¿ç”¨å…¶å„é˜¶ç§¯åˆ†

- è¿ç»­åŒèƒšä½†ä¸å¾®åˆ†åŒèƒšä¸è§£æåŒèƒš. $x^3$ 

- å¾®åˆ†åŒèƒšä½†ä¸è§£æåŒèƒš. å…‰æ»‘ä½†å¤„å¤„ä¸è§£æå‡½æ•°ä¸­å– $#d f != 0$ çš„éƒ¨åˆ†å¾—åˆ°å±€éƒ¨å¾®åˆ†åŒèƒš. å±€éƒ¨åˆ°å…¨å±€ by ç”¨ $x/(1-x)$ å¾—åˆ° $(-1,1) -> â„$ çš„è§£æåŒèƒš