#import "/module/module.typ": *
#show: module

#tag("tensor-induced-quadratic-form") 
#indent[
  Derive the quadratic form $⟨ , ⟩$ of the vector space to the quadratic form $⟨ , ⟩^(⊗ k)$ of the tensor space 
  $
    ⟨v_1 ⊗ ⋯ ⊗ v_k , w_1 ⊗ ⋯ ⊗ w_k⟩ = ⟨v_1,w_1⟩ ⋯ ⟨v_k,w_k⟩
  $  
  Iterate through all $i_1 ,…, i_k$ orthonormal bases $e_(i_1) ⊗ ⋯ ⊗ e_(i_k)$ with $(e_(i_1) ⊗ ⋯ ⊗ e_(i_k))^2 = e_(i_1)^2 ⋯ e_(i_k)^2$, to obtain the signature

  Alternation 
  $
    ⟨v_1 ∧ ⋯ ∧ v_k , w_1 ∧ ⋯ ∧ w_k⟩ = det ⟨v_i,w_j⟩ 
  $
  Iterate through all $i_1 < ⋯ < i_k$, orthonormal bases $e_(i_1) ∧ ⋯ ∧
  e_(i_k)$ with $(e_(i_1) ∧ ⋯ ∧ e_(i_k))^2 = e_(i_1)^2 ⋯ e_(i_k)^2$, to obtain the signature

  let $v,w ∈ ℝ^n$. $v,w$ span $ℝ^2$ <==> $v ∧ w != 0$
]
*Abbreviation* $v w := ⟨ v , w ⟩, v^2 := ⟨ v , v ⟩, |v| := (v^2)^(1/2)$

#tag("quadratic-form-inequality-Euclidean") Inner product inequality (Euclidean). $0 <= (v ∧ w)^2 = det mat(v^2, v w; w v, w^2) = v^2 w^2 - (v w)^2$. i.e. $(v w)^2 <= v^2 w^2$ or $v w <= |v| |w|$

#tag("triangle-inequality-Euclidean") Triangle inequality (Euclidean)
  - $|v + w| <= |v| + |w|$ 

    *Proof*
      $
        (v+w)^2 &= v^2 + 2 v w + w^2 \
        &>= v^2 + 2 |v| |w| + w^2 \
        &= (|v| + |w|)^2
      $
  - $|v - w| >= stretch(|, size: #120%)|v| - |w|stretch(|, size: #120%)$

    *Proof*
      $
        |v| &<= |v-w| + |w| \
        |w| &<= |v-w| + |v|
      $
#tag("Euclidean-space-topology") Euclidean $ℝ^d$ topology. $f : ℝ^d -> ℝ^d'$ is continuous at $a ∈ ℝ^d$ :=
  $
    forall ε > 0, exists δ > 0, forall x : |x - a| < δ, |f(x) - f(a)| < ε
  $
let $A ⊂ ℝ^d$

#let closed(x) = math.macron(x)
#let Closed(x) = math.overline(x)

#tag("closure") Closure := $closed(A) = {x ∈ ℝ^d : inf_(x ∈ A) |x-a| = 0}$

#tag("closed-set") Closed set := $closed(A) = A$

(open) closed(𝔹) $𝔹(a,r) := {x ∈ ℝ^d : |x - a| < r}$

#tag("open-set") Open set $U ⊂ ℝ^d$ := $forall x ∈ U, exists r > 0, 𝔹(x,r) ⊂ U$

$A$ open <==> $A^∁$ closed 

#let I = c-bf("I","#919191")
#let J = c-bf("J","#919191")

#tag("interval") Interval refers to a subset $I$ of $ℝ$ with property that the order is uninterrupted
$ 
  And_(a,b ∈ I \ a <= b) And_(x ∈ ℝ \ a <= x <= b) x ∈ I 
$
#tag("best-interval-decomposition") The optimal interval decomposition of $A ⊂ ℝ$
#indent[
  def $"Interval" ⊂ Subset(ℝ)$ as the set of all intervals, including open, closed, half open half closed, single point

  def $#J (A) := {I ⊂ A : I ∈ "Interval"}$

  Due to the existence of single-point intervals, $#J != ∅$ and $⋃ #J = A$

  $#J (A)$ has a $⊂$ #link(<linear-order>)[linear order chain]. Taking $⋃$ for each maximal linear order chain will continue to yield intervals. The set of these intervals is denoted as $#I (A)$

  $#I (A) != ∅$ and $⨆ #I (A) = A$  

  The intervals in $#I$ are disjoint, and the decomposition method is unique, so these intervals form the optimal interval decomposition of $A$

  - When $|#I (A)| = 1$, $A$ is an interval, connected
  - When $|#I (A)| > 1$, $A$ is not connected. *Example* $ℝ ∖ 0 = ℝ_(< 0) ⊔ ℝ_(>  0), ℚ = ⨆ _(x ∈ ℚ) {x}$

  If $A$ is a closed set, then the intervals in $#I (A)$ are all closed intervals
]
recall the $⊂$ #link(<linear-order>)[] #link(<nested-closed-interval-theorem>)[intersection of nested closed intervals is non-empty]

#tag("bounded-closed-interval-is-compact") Bounded closed interval of $ℝ$ ==> #link(<compact>)[]

*Proof* 
#let B = c-bf("B","#919191")
#let C = c-bf("C","#919191")
#indent[
  let $#B$ be a #link(<net>)[net] of $A$. let $B in #B$

  Since $A ⊂ ℝ$ is bounded and closed, $closed(B) ⊂ A$

  Take the optimal closed interval decomposition $closed(B) = ⨆ #I (closed(B))$

  For all decomposed closed intervals of $B in #B$, consider any $⊂$ maximal linear order chain #link(<maximal-linear-order>)[] $#C$

  According to #link(<nested-closed-interval-theorem>)[], the intersection of a nested set of closed intervals in the $⊂$ linear order is a non-empty closed interval $⋂ #C != ∅$

  Similar to the proof of #link(<closed-interval-net-theorem>)[], prove that $⋂ #C$ is the smallest closed interval, thus $subset$ every $B in #B$
]
#tag("compact-imply-subsequence-converge") $A$ compact ==> sequence ${x_n} ⊂ A$ has a convergent subsequence. The same applies to nets

*Proof* 
#indent[
  $B_n = {x_n,x_(n+1),...}$ forms a net $#B$
  
  $A$ compact ==> $⋂_(n ∈ ℕ) closed(B)_n != ∅$
  
  let $x ∈ ⋂_(n ∈ ℕ) closed(B)_n$
  
  use the definition of closure $closed(B)_n$ 
  
  $ 
    x in closed(B)_n 
    <==> forall ε_n > 0, exists i_n > i_(n-1), |x_(i_n) - x| < ε_n 
  $

  let $ε_n -> 0$ 
  
  ==> $forall ε > 0, exists N in ℕ, forall n > N, |x_(i_n) - x| < ε$
]
- Unit closed ball $closed(𝔹)^n := {x ∈ ℝ^n : x^2 <= 1}$
- Unit sphere $𝕊^(n-1) := {x ∈ ℝ^n : x^2 = 1}$

#tag("circle-is-compact") $𝕊^1$ compact

*Proof* $e^(#i θ) : ℝ -> 𝕊^1$ is continuous
#indent[
  $𝕊^1$ is continuously isomorphic to $ℝ/ℤ$ (#link(<quotient-topology>)[]) is continuously isomorphic to $closed(𝔹)^1/𝕊^0$ i.e. $[-1,1] = closed(𝔹)^1$ collapsing endpoints ${-1,1} = 𝕊^0$ (quotient-topology)

  $closed(𝔹)^1 = [-1,1]$ bounded closed interval compact ==> quotient $𝕊^1 = closed(𝔹)^n/𝕊^0$ compact. by #link(<quotient-topology-preserve-compact>)[quotient preserves compact]
]
#tag("closed(𝔹)-sphere-is-compact") 

*Proof* 
#indent[
  $closed(𝔹)^1, 𝕊^1$ compact. Inductive hypothesis $closed(𝔹)^n, 𝕊^n$ compact

  - $closed(𝔹)^(n+1)$ compact
  #indent[
    $
      f : dmat( delim: #none ,
        𝕊^n × [0,1], ⟶, closed(𝔹)^(n+1);
        (x,r), ⟿, r ⋅ x
      )
    $
    (Draw a picture) continuous. Isomorphism is obtained after quotienting the origin $0 ∈ ℝ^(n+1)$

    $𝕊^n × [0,1]$ compact. by #link(<product-topology-preserve-compact>)[]

    $(𝕊^n × [0,1])/{0 ∈ ℝ^(n+1)} ≃ closed(𝔹)^(n+1)$ compact
  ]
  - $𝕊^(n+1)$ compact
  #indent[
    Constructing $𝕊^(n+1)$ from $𝕊^n$ using polar coordinates, after quotient, we get $𝕊^(n+1)$ compact

    Another method $closed(𝔹)^(n+1)$ the boundary $𝕊^n$ collapses to a point to get $closed(𝔹)^(n+1)/𝕊^n ≃ 𝕊^(n+1)$ compact
    
    *Proof* 
    #indent[
     $1/(1 - |x|^2) x : 𝔹^(n+1) <-> ℝ^(n+1)$ maps the sphere $𝕊(|x|)$ to the sphere $𝕊^((|x|)/(1 - |x|^2))$ and $r/(1 - r^2) : [0,1) <-> ℝ_(>= 0)$

     Stereographic projection $ℝ^(n+1) <-> 𝕊^(n+1) ∖ N$

     The composite mapping $𝔹^(n+1) -> 𝕊^(n+1) ∖ N$ plus the mapping $∂ closed(𝔹)^(n+1) = 𝕊^n$ mapping to $N$, the resulting $closed(𝔹)^(n+1) -> 𝕊^(n+1)$ mapping is still continuous, and after quotient it is a bijection
    ]
  ]
]
Projective space (Euclidean) compact. *Proof* $ℝℙ^n := ℝ^(n+1)/{k x} ≃ 𝕊^n/{± x}$ 

Similarly $ℂℙ^n$ (and $ℍℙ,𝕆ℙ$)

#tag("Euclidean-set-distance") $|A| := sup_(x,y ∈ A) |x-y|$ 

- #tag("bounded") bounded := $|A| < ∞$ 
- #tag("unbounded") unbounded := $|A| = ∞$ 

$|A|$ is $SO(n) ⋊ ℝ^n$ invariant

$ℝ ⊔ {∞} ≃ 𝕊^n$ by stereographic projection

Translation does not change the infinity $∞$ of $ℝ^n ⊔ {∞}$ (but only a conformal mapping of $ℝ^n ⊔ {∞} ≃ 𝕊^n$, conformal group $SO(1,n)$) 

in Euclidean topology of $ℝ^n ⊔ {∞} ≃ 𝕊^n$
- Bounded <==> away from $∞$ <==> $∞ ∉ closed(A)$
- Unbounded <==> $∞ ∈ closed(A)$

#tag("Euclidean-space-compact-iff-bounded-closed") $A ⊂ ℝ^n$ compact <==> $A$ is a bounded closed set 

*Proof*
#indent[
  - <==
  #indent[
    The bounded closed set $A$ of $ℝ^n$ corresponds to a closed set of $ℝ^n ⊔ {∞}$ and does not include $∞$

    $𝕊^n$ compact + #link(<closed-set-in-compact-space-is-compact>)[] ==> $A$ is compact in $𝕊^n$

    From $ℝ^n ⊔ {∞}$ topology, restrict back to subspace $ℝ^n$ topology + $A subset ℝ^n$

    Get $A$ compact
  ]
  - ==>
  #indent[
    - Closed set
    #indent[
      let $x ∈ closed(A)$

      $𝔹(x,r) ∩ A$ forms a net of $A$. Note that it is possible that $x ∉ 𝔹(x,r) ∩ A$

      - compact ==> $∅ != ⋂_(r > 0) closed(𝔹)(x,r) ∩ A ⊂ A$

      - $⋂_(r > 0) closed(𝔹)(x,r) = x$

      ==> $∅ != {x} ∩ A ==> x in A$
    ]
    - Bounded
    #indent[
      The open ball of $ℝ^d$ does not contain $∞$. The open ball family ${𝔹(x,r) ⊂ ℝ^n : (x ∈ A) and (r > 0)}$ covers $A$. Take #link(<compact-finite-open-cover>)[finite cover], still does not contain $∞$
    ]
  ]
]
let $#B$ be net of $ℝ^n$

#tag("nested-closed-set-theorem") The intersection of nested bounded closed sets of $ℝ^n$ is non-empty. The intersection result is also a closed set. It can be understood as the minimal element of $⊂$ linear order chain nested closed sets

#tag("closed-net-theorem") The intersection of a net of bounded closed sets of $ℝ^n$ is non-empty
*Proof*
#indent[
  Map the closed set of $ℝ^n$ to the closed set of $ℝ^n ⊔ {∞} ≃ 𝕊^n$, $𝕊^n$ is compact, so the intersection of nested closed sets or the intersection of a net of closed sets is non-empty. Boundedness makes it not converge to $∞$
]
#tag("limit-distance-vanish-net") := $lim_(B ∈ #B) |B| = 0$ 

or $forall ε > 0, exists B ∈ #B, |B| < ε$. The tail of the net is bounded

A net can be composed of tails $B_n = {x_n,x_(n+1),...}$ 

#tag("Cauchy-completeness-Euclidean") 
#indent[
  in $ℝ^n$, limit-distance-vanish net converges to a point
  
  According to the closed set net theorem ==> let $x in ⋂_(B ∈ #B) closed(B) != ∅$

  limit-distance-vanish $lim_(B ∈ #B)|B| = 0$ ==> $⋂_(B ∈ #B) closed(B) = {x}$
]
Some infinite-dimensional linear spaces e.g. #link(<Lebesgue-integrable>)[] $L^1$, bounded closed sets cannot be compact but still satisfy limit-distance-vanish net converging to a point

According to induction, finite summation is associative and commutative. But this does not guarantee infinite summation i.e. 

let
- Rearrangement $f : ℕ <-> ℕ$ 
- $x_n = a_1 + ⋯ + a_n$ converges to $x$
Then $y_n = a_(f(1)) + ⋯ + a_(f(n))$ may not converge or converge to other value $y != x$

compare
- $sum 1/n = ∞$
- $sum (-1)^(n+1) 1/n = log(1+1) = log(2)$ 
Convergence (not ==>) Absolute convergence

let $a_n$ be a sequence $ℕ -> ℝ$

- $sum_(.. ∞) a_n$ converges ==> $lim_(n -> ∞) a_n = 0$
  
  *Proof* $forall ε > 0, exists N in ℕ, forall n > N, abs(sum_(i = 1 .. n) a_i - a) < ε/2$ 

   ==> By the triangle inequality 
   
   $ |a_n| = abs(sum_(i = 1 .. n+1) a_i - sum_(i = 1 .. n) a_i) <= abs(sum_(i = 1 .. n+1) a_i - a) + abs(sum_(i = 1 .. n) a_i - a) < ε $
- $lim_(n -> ∞) a_n != 0$ ==> $sum_(.. ∞) a_n$ does not converge

Any sequence $x_n$ can define $a_n = x_n - x_(n-1)$ such that $x_n = a_1 + ⋯ + a_n$

Rearrangement $f : ℕ <-> ℕ$ does not change the tail behavior of the sequence $lim_(n -> ∞) a_(f(n)) = lim_(n -> ∞) a_n$

If $a_n >= 0$, $sum a_n$ rearrangement invariant

*Proof* 
#indent[
  $sum a_n < ∞ ==> forall ε > 0, exists N ∈ ℕ, forall m > ℕ, sum a_n - epsilon < sum_(n=0..m) a_n <= sum a_n$

  $N' := max {f^(-1)(1) ,…, f^(-1)(N)}$

  ==> ${1 ,…, N} ⊂ {f(1) ,…, f(N')}$

  ==> $forall M > N', sum a_n - epsilon <= sum_(n=0..N) a_n <= sum_(n=0..M) a_(f(n)) <= sum a_n$ (by $a_n >= 0$)

  ==> $lim_(M -> ∞) sum_(n=0..M) a_(f(n)) = sum a_n$
]
def
$
  a_n^+ &:= "switch"(a_n) cases(>= 0 => a_n , < 0 => 0) \

  a_n^- &:= "switch"(a_n) cases(>= 0 => 0 , < 0 => - a_n) \

  a_n^+,a_n^- &>= 0 \

  a_n &= a_n^+ - a_n^-
$
$ sum |a_n| < ∞ <==> sum a_n^+, sum a_n^- < ∞ $

#tag("series-rearrangement-absolutely-convergence-real") Absolute convergence $sum_(.. ∞) |a_n|$ ==> $sum_(.. ∞) a_n$ converges and rearrangement invariant 
  
*Proof* $a_n = a_n^+ - a_n^-$ and use operation of convergent sequence 
  $
    lim sum_(.. N) a_n 
    
    = lim sum_(.. N) a_n^+ - lim sum_(.. N) a_n^-
  $
$sum a_n^+ = ∞$ and $sum a_n^- < ∞$ ==> $sum a_n = +∞$ and rearrangement invariant

*Question* The case of $l^2$ norm $(sum |a_n|^2)^(1/2)$ reduce to $b_n = |a_n|^2$?

The last possibility

#tag("series-rearrangement-real") 
#indent[
  let $lim_(n -> ∞) a_n = 0$ and $sum a_n^+ = sum a_n^- = ∞$

  $exists f : ℕ <-> ℕ, sum a_(f(n))$
  - Converges to $ℝ,+∞,-∞$
  - Does not converge to $ℝ,+∞,-∞$ 
]
*Example*
- Convergent case $a_n = (-1)^(n+1) 1/n$
- Divergent case $a_n = (-1)^n$

*Proof* 
#indent[
  - Converges to $A ∈ ℝ$
  #indent[
    $p_1 := inf { p ∈ ℕ : A < sum_(.. p) a_n^+ }$. Meaning: $p_1$ is the smallest natural number that makes the positive summation greater than $A$

    $q_1 := inf { q ∈ ℕ : A > sum_(.. p_1) a_n^+ - sum_(.. q) a_n^- }$. Meaning: $q_1$ is the smallest natural number that makes the negative summation less than $A$

    $p_2 := inf { p ∈ ℕ : A > sum_(.. p) a_n^+ - sum_(.. q_1) a_n^- }$

    And so on, exhaust all $a_n$

    Rearrange $a_1,a_2,...$ to 
    $
      a_1^+ ,…, a_(p_1)^+ \ - a_1^- ,…, - a_(q_1)^- \ a_(p_1 + 1)^+ ,…, a_(p_2)^+ \
      ⋮
    $
    According to the definition of $p_(N+1)$
    $
      0 

      &< (sum_1^(p_(N+1)) a_n^+ - sum_1^(q_N) a_n^-) - A \

      &<= (sum_1^(p_(N+1)) a_n^+ - sum_1^(q_N) a_n^-) 
      - (sum_1^(p_(N+1) - 1) a_n^+ - sum_1^(q_N) a_n^-) \

      &= a_(p_(N+1))^+
    $
    According to the definition of $q_(N+1)$
    $
      0 
      
      < (sum_1^(p_(N+1)) a_n^+ - sum_1^(q_N ,…, q_(N+1) - 1) a_n^-) - A 
      
      <= a_(p_(N+1))^+
    $
    And so on
    $
      - a_(q_(N+1))^- 

      <= (sum_1^(p_(N+1) ,…, p_(N+2) - 1) a_n^+ - sum_1^(q_(N+1)) a_n^-) - A 

      < 0
    $
    $lim_(n -> ∞) a_n = 0 ==> lim_(N -> ∞) a_(p_(N))^+ = lim_(N -> ∞) a_(q_N)^- = 0$

    ==> $lim_(N -> ∞) sum_(.. N) a_n = A$
  ]
  - Converges to $+∞$
  #indent[
    In the handling of $A ∈ ℝ$
    
    Change $A < sum_1^⋯ a_n^+ - sum_1^⋯ a_n^-$ to $N < sum_1^⋯ a_n^+ - sum_1^⋯ a_n^-$

    Change $A > ⋯$ to $N > ⋯$
  ]
  - Does not converge to $ℝ,+∞,-∞$
  #indent[
    Change $A < ⋯$ to $1 < ⋯$

    Change $A > ⋯$ to $-1 > ⋯$
  ]
]
Series in $ℝ^d$ that are rearrangement invariant are also absolutely convergent series

$sum a_n$ converges ==> $lim_(n -> ∞) a_n = 0$

#tag("series-rearrangement-absolutely-convergence") 
#indent[
  let $a_n$ be a $ℕ -> ℝ^d$ sequence

  $sum |a_n| < ∞$ ==> $sum a_n$ converges and is rearrangement invariant 
]
*Proof* 
#indent[
  - $sum a_n$ converges. by using the triangle inequality $abs(sum_(N+1)^∞ a_n) <= sum_(N+1)^∞ |a_n|$ and $ℝ^d$ #link(<Cauchy-completeness-Euclidean>)[Cauchy sequence converges]

  - Rearrangement invariant
  #indent[
    $forall ε > 0, exists N ∈ ℕ, (abs(sum_(.. N) a_n - A) < ε/2) and (sum_(N+1)^∞ |a_n| < ε/2)$

    $N' := max {f^(-1)(1) ,…, f^(-1)(N)}$

    ${1 ,…, N} ⊂ {f(1) ,…, f(N')}$

    $forall M > N', 
    abs(sum_(.. M) a_(f(n)) - A) 
    <= abs(sum_(.. N) a_n - A) + sum_(N+1)^∞ |a_n| 
    < ε$
  ]
]
Now consider the case where $sum a_n$ is not absolutely convergent

def $V := { x ∈ ℝ^d : sum |⟨ a_n, x ⟩| < ∞ }$

From the triangle inequality or the equivalence of $1$-norm, $2$-norm, $∞$-norm of $ℝ^d$
- $V$ is a linear subspace
- $V = ℝ^d ==> sum |a_n| < ∞$

let $V != ℝ^d$. The $V$ component of $sum a_n$ is absolutely convergent

Consider the $V^⟂$ component of $sum a_n$

#tag("series-rearrangement") 
#indent[
  let $x ∈ V^⟂$ 

  - $sum ⟨ a_n , x ⟩^+ = ∞$ and $sum ⟨ a_n , x ⟩^- < ∞$ ==> $sum a_n$ converges to $∞$ in the $x$ component, rearrangement invariant \
  - $sum ⟨ a_n , x ⟩^+ = sum ⟨ a_n , x ⟩^- = ∞$. $sum a_n$ is rearrangement unstable in the $x$ component
]

The *positive* linear combination $k a_n + k' a'_n$ with $sign(k) = sign(k')$ of sequences with the same convergence pattern preserves their convergence pattern