#import "/module/module.typ": *
#show: module

#tag("real-exponential")
#indent[
  If the exponent is a natural number, then $a^(n+m) = a^(n) a^m$. It can be simply generalized to rational numbers

  For the exponent being a real number, define the exponential function $x ‚áù a^x$ as satisfying $a^(x+y) = a^x a^y$ and $a^1 = a$

  Assume $f(x) = a^x$ is analytic. Power series expansion of $f(x+y) = f(x)f(y)$ (requires commutativity of $‚Ñù,‚ÑÇ,‚ÑÇ_"split"$?)

  Expand both sides
  $
    sum (f^((n)) (0))/n! (x+y)^n &= sum (f^((n)) (0))/n! x^n sum (f^((n)) (0))/n! y^n \

    sum_n sum_(i+j=n) (f^((n)) (0))/n! n!/(i! j!) x^i y^j &=  sum_n sum_(i+j=n) (f^((i)) (0))/i! (f^((j)) (0))/j! x^i y^j
  $
  Let the coefficients be the same $forall n, forall i+j=n, f^((n)) (0) = f^((i)) (0) f^((j)) (0)$ \
  ==>
  - $forall n,  f^((n)) (0) = f^((n)) (0) f^((0)) (0) ==> f^((0)) (0) = 1$ 
  - $forall n, f^((n)) (0) = (f^((1)) (0))^n$
  ==> 
  $
    f(x) = sum ((f^((1)) (0))/n! x)^n
  $

  #tag("natural-exponential") def $e^x = exp x = sum 1/n! x^n : ‚Ñù -> (0,‚àû)$ with $e^1 = exp(1) = sum 1/n! = e$ #link(<natural-constant>)[]

  from the series, we can see that, differential $(#d)/(#d x) (e^x) = e^x > 0$ ==> $e^x$ exists #link(<inverse-analytic>)[]

  #tag("natural-logarithm") def $log = exp^(-1) : (0,‚àû) -> ‚Ñù$. $(#d)/(#d x) log x = 1/x$

  for $a > 0$, def $f^1 (0) := log a in ‚Ñù$

  for $a$, def $f^1 (0) := log a in ùïÇ$
  $
    a^1 &= f(1) \
    &= sum 1/n! (log a)^n \
    & = exp log a \
    & = a \

    a^x &= f(x) \
    &= sum 1/n! (log a ‚ãÖ x)^n \
    &= exp (x log a)
  $
]
#tag("power-function") Defining the exponential function means that for each $a in ‚Ñù$, each real exponent $x$ is defined, and thus the power function $a ‚áù a^x$ is also defined, or rewritten as $x ‚áù x^a$

It can also be expressed as $x^a = exp(a log x)$

#tag("Euler-formula")

  - $‚ÑÇ$
  $
    exp z &= cos z + #i sin z \
    #i &‚âÉ mat(,-1;1) ‚àº so(2)
  $
  - $‚ÑÇ_"split"$
  $
    exph z &= cosh z + #i-split sinh z \
    #i-split &‚âÉ mat(,1;1) ‚àº so(1,1)
  $